coq/coq/Translation.v
@@ -7,6 +7,13 @@ Require Import Sorting.Permutation.
 Require Import Sorting.Sorted.
 Require Export Infrastructure.
 
+Lemma TEI_dup : forall (ll:tindex) (At Bt Ct Ct' At':ttyp),
+     rec_typ Ct ->
+      (   (  Tlookup  ll   Ct  = Some  At'   /\  eqIndTypTarget At' At )    \/   Tlookup  ll   Ct  = None  )  ->
+     eqIndTypTarget At Bt ->
+     eqIndTypTarget (ttyp_rcd ll Bt  (ttyp_rcd ll At Ct) ) Ct' ->
+     eqIndTypTarget (ttyp_rcd ll At  (ttyp_rcd ll Bt Ct) ) Ct'.
+Admitted.
 
 Lemma lookup_wf_typ_1 : forall l T At l',
     Tlookup l' (ttyp_rcd l T At) = Tlookup l' At \/ l = l'.
@@ -144,6 +151,12 @@ Proof with eauto.
   introv HE HR. gen A. inductions HR; intros; inverts* HE.
 Qed.
 
+Lemma eqIndTypTarget_rec_typ_2 : forall A B,
+    eqIndTypTarget A B -> rec_typ A -> rec_typ B.
+Proof with eauto.
+  introv HE. induction HE; intros... inverts* H.
+Qed.
+
 Lemma TEI_refl : forall At,
     wf_typ At -> eqIndTypTarget At At.
 Proof with eauto.
@@ -176,7 +189,6 @@ Lemma eqIndTypTarget_arrow_inv_3 : forall A B C,
 Proof with eauto; try solve_by_invert.
   introv HE. inductions HE...
   - forwards* (?&?&?): IHHE...
-  - forwards* (?&?&?): IHHE2...
 Qed.
 
 Lemma TEI_symm : forall A B,
@@ -229,14 +241,15 @@ Proof with eauto.
     +
       econstructor...
       right; unify_lookup; tassumption.
-  - inverts* IHHS2. inverts H5. inverts H6.
-    unify_lookup.
-    econstructor... econstructor...
-    left; split*. eauto using TEI_trans.
-    left; split. unify_lookup. eauto using TEI_trans, TEI_symm.
-    econstructor...
-    left; split. unify_lookup. eauto using TEI_trans, TEI_symm.
-    Unshelve. all: eauto.
+  (* - inverts* IHHS2. inverts H5. inverts H6. *)
+  (*   unify_lookup. *)
+  (*   econstructor... econstructor... *)
+  (*   left; split*. eauto using TEI_trans. *)
+  (*   left; split. unify_lookup. eauto using TEI_trans, TEI_symm. *)
+  (*   econstructor... *)
+  (*   left; split. unify_lookup. eauto using TEI_trans, TEI_symm. *)
+      (*   Unshelve. all: eauto. *)
+      Unshelve. all: eauto.
 Qed.
 
 Lemma eqindtyptarget_wf_typ_2 : forall At Bt,
@@ -285,15 +298,15 @@ Proof with eauto using TEI_symm, TEI_refl, TEI_trans.
       econstructor...
     all: eauto using eqindtyptarget_wf_typ_1, eqindtyptarget_wf_typ_2,
         wf_rcd_concat, rcd_typ_concat_1, rcd_typ_concat_2, rcd_typ_concat_3.
-  - forwards* (?&?&?): IHHE2. inverts keep H1. inverts H9.
-    unify_lookup; lookup_concat ll H11...
-    all: exists; split.
-    1,3,5,7: econstructor; try solve [right*]; try solve [left*].
-    1-4: econstructor; try solve [right*]; try solve [left*]...
-    all: applys TEI_dup H2.
-    all: try solve [right*]; try solve [left*]...
-    all: eauto using eqindtyptarget_wf_typ_1, eqindtyptarget_wf_typ_2,
-        wf_rcd_concat, rcd_typ_concat_1, rcd_typ_concat_2, rcd_typ_concat_3.
+  (* - forwards* (?&?&?): IHHE2. inverts keep H1. inverts H9. *)
+  (*   unify_lookup; lookup_concat ll H11... *)
+  (*   all: exists; split. *)
+  (*   1,3,5,7: econstructor; try solve [right*]; try solve [left*]. *)
+  (*   1-4: econstructor; try solve [right*]; try solve [left*]... *)
+  (*   all: applys TEI_dup H2. *)
+  (*   all: try solve [right*]; try solve [left*]... *)
+  (*   all: eauto using eqindtyptarget_wf_typ_1, eqindtyptarget_wf_typ_2, *)
+  (*       wf_rcd_concat, rcd_typ_concat_1, rcd_typ_concat_2, rcd_typ_concat_3. *)
     Unshelve. all: econstructor.
 Qed.
 
@@ -632,12 +645,12 @@ Proof with eauto using translate_to_record_types.
     + forwards*: IHHEA1. + forwards*: IHHEA2.
   - applys* TEI_symm. admit.
   - simpl... admit.
-  - admit.
-  (* - simpl... applys TEI_trans. applys TEI_comm. applys H. applys* TEI_rcd. applys* TEI_rcd. *)
-    (* induction* Ct. simpl... *)
+(*   - admit. *)
+(*   (* - simpl... applys TEI_trans. applys TEI_comm. applys H. applys* TEI_rcd. applys* TEI_rcd. *) *)
+(*     (* induction* Ct. simpl... *) *)
 
-  (* - simpl... applys TEI_trans. applys TEI_dup. applys* TEI_rcd. applys* TEI_rcd. *)
-    (* induction* Ct. simpl... *)
+(*   (* - simpl... applys TEI_trans. applys TEI_dup. applys* TEI_rcd. applys* TEI_rcd. *) *)
+(*     (* induction* Ct. simpl... *) *)
 Admitted.
 (* Qed. *)
 
@@ -704,4 +717,3 @@ Admitted.
 
 Lemma subtypespec_andr : forall A B, subtype_wrt_lookup |[typ_and A B]| |[B]|.
 Admitted.
-2
